---
title: "A2_solution"  
author: "Reinforcement Learning Study"  
date: "`r Sys.Date()`"  
output:   
  pdf_document:  
    latex_engine: xelatex
    highlight: haddock  
    keep_tex: true  
    includes:
      #in_header: rmd-pdf-support/latex-topmatter.tex
    # pandoc_args: [
    #  "-V", "classoption=twocolumn"
    # ]
    toc: true   
    toc_depth: 2  
    # number_sections: true  
monofont: Consolas
smaller: yes
classoption: a4paper
---

```{r setup, include=FALSE}
knitr::opts_chunk$set(echo = TRUE)
knitr::opts_chunk$set(background = '718CBA')  
```

\newpage

# Exercise

## Exercise 1



*Show that* $\mathbb{P}(A \mid B \cap C)\mathbb{P}(B \mid C)=\mathbb{P}(A \cap B \mid C)$


\vspace{20pt}

$\mathbb{P}(A \mid B \cap C)\mathbb{P}(B \mid C)=\frac{\mathbb{P}(A \cap (B \cap C))}{\mathbb{P}(B \cap C)} \times \frac{\mathbb{P}(B \cap C)}{\mathbb{P}(C)}$

$\,\,\,\,\,\,\,\,\,\,\,\,\,\,\,\,\,\,\,\,\,\,\,\,\,\,\,\,\,\,\,\,\,\,\,\,\,\,\,\,\,\,\,\,\,\,\,\,\,\,\,\,\,\,\,\,\,\,\,=\frac{\mathbb{P}(A \cap B \cap C)}{\mathbb{P}(C)}$

$\,\,\,\,\,\,\,\,\,\,\,\,\,\,\,\,\,\,\,\,\,\,\,\,\,\,\,\,\,\,\,\,\,\,\,\,\,\,\,\,\,\,\,\,\,\,\,\,\,\,\,\,\,\,\,\,\,\,\,=\frac{\mathbb{P}((A \cap B) \cap C)}{\mathbb{P}(C)}$

$\,\,\,\,\,\,\,\,\,\,\,\,\,\,\,\,\,\,\,\,\,\,\,\,\,\,\,\,\,\,\,\,\,\,\,\,\,\,\,\,\,\,\,\,\,\,\,\,\,\,\,\,\,\,\,\,\,\,\,=\mathbb{P}(A \cap B \mid C)$
\vspace{15pt}

$\therefore \,\,\, \mathbb{P}(A \mid B \cap C)\mathbb{P}(B \mid C)=\mathbb{P}(A \cap B \mid C)$



\newpage
## Exercise 2


*X~U(10,20), then what is F(10)? and F(15)?*

\vspace{20pt}

*X~U(10,20)*

\vspace{10pt}

\[f(x)=
\begin{Bmatrix}
\frac{1}{10} \,\,(10\leq x\leq 20) \\ \\
0 \,\,\,\,\,\,\,\,\,\,\,\,\, otherwise
\end{Bmatrix}
\]
\vspace{10pt}
\[F(x)=
\begin{Bmatrix}
0 \,\,\,\,\,\,\,\,\,\,\,\,\,\,\,\,\,(10\leq x) \\\\ \frac{x-10}{10} \,\,\,\,\,\,\,(10\leq x \leq 20) \\\\1 \,\,\,\,\,\,\,\,\,\,\,\,\,(x>20)
\end{Bmatrix}
\]


\begin{figure}[ht]
\centering
   \includegraphics[width=8.5cm]{graph}
   \hfil
\caption{F(x) graph}
\label{Fig1.}
\end{figure}

\vspace{20pt}



$F(10)=0$
\vspace{10pt}

$F(15)=\frac{15-10}{10}$

$\,\,\,\,\,\,\,\,\,\,\,\,\,\,\,\,\,\,=\frac{1}{2}$

\vspace{10pt}
$\therefore\,\, F(10)=0,\,\,F(15)=\frac{1}{2}$

\newpage


## Exercise 3

*Prove that pdf*$\rightarrow$*cdf*

\vspace{20pt}

$F(x)=\int_{-\infty}^{x}f(x)\,\,dx$

i) $if \,\,\, x<0, \,\,\,then \,\,\,\,f(x)=0, \,\,\,so \,\,\,F(x)=0$
\vspace{10pt}

ii) $if \,\,\, x\geq0, \,\,\,then \,\,\,F(x)=\int_{-\infty}^{x}f(x)\,\,dx$

$\,\,\,\,\,\,\,\,\,\,\,\,\,\,\,\,\,\,\,\,\,\,\,\,\,\,\,\,\,\,\,\,\,\,\,\,\,\,\,\,\,\,\,\,\,\,\,\,\,\,\,\,\,\,\,\,\,\,\,\,\,\,\,\,\,\,\,\,\,\,\,\,\,=\int_{-\infty}^{0}0\,\,dx+\int_{0}^{x}\lambda e^{-\lambda x}\,\,dx$

$\,\,\,\,\,\,\,\,\,\,\,\,\,\,\,\,\,\,\,\,\,\,\,\,\,\,\,\,\,\,\,\,\,\,\,\,\,\,\,\,\,\,\,\,\,\,\,\,\,\,\,\,\,\,\,\,\,\,\,\,\,\,\,\,\,\,\,\,\,\,\,\,\,=[-e^{\lambda x}]_{0}^{x}$

$\,\,\,\,\,\,\,\,\,\,\,\,\,\,\,\,\,\,\,\,\,\,\,\,\,\,\,\,\,\,\,\,\,\,\,\,\,\,\,\,\,\,\,\,\,\,\,\,\,\,\,\,\,\,\,\,\,\,\,\,\,\,\,\,\,\,\,\,\,\,\,\,\,=-e^{-\lambda x}+1$

\vspace{10pt}

$\therefore\,\,\,F(x)=1-e^{-\lambda x}$




\newpage
## Exercise 4

*Show that EX=*$1/\lambda$

\vspace{20pt}

$\mathbb{E}X=\int_{-\infty}^{\infty}xf(x)\,\,dx=\int_{-\infty}^{0}xf(x)\,\,dx+\int_{0}^{\infty}xf(x)\,\,dx$

$\,\,\,\,\,\,\,\,\,\,\,\,\,\,\,\,\,\,\,\,\,\,\,\,\,\,\,\,\,\,\,\,\,\,\,\,\,\,\,\,\,\,\,\,\,\,\,\,\,\,\,\,\,=\int_{0}^{\infty}x\lambda e^{-\lambda x}\,\,dx$

$\,\,\,\,\,\,\,\,\,\,\,\,\,\,\,\,\,\,\,\,\,\,\,\,\,\,\,\,\,\,\,\,\,\,\,\,\,\,\,\,\,\,\,\,\,\,\,\,\,\,\,\,\,=\int_{0}^{\infty}\lambda xe^{-\lambda x}\,\,dx$

$\,\,\,\,\,\,\,\,\,\,\,\,\,\,\,\,\,\,\,\,\,\,\,\,\,\,\,\,\,\,\,\,\,\,\,\,\,\,\,\,\,\,\,\,\,\,\,\,\,\,\,\,\,=[xe^{-\lambda x}]_{0}^{\infty}-\int_{0}^{\infty}-e^{-\lambda x}\,\,dx$

$\,\,\,\,\,\,\,\,\,\,\,\,\,\,\,\,\,\,\,\,\,\,\,\,\,\,\,\,\,\,\,\,\,\,\,\,\,\,\,\,\,\,\,\,\,\,\,\,\,\,\,\,\,=(0-0)+\int_{0}^{\infty}e^{-\lambda x}\,\,dx$

$\,\,\,\,\,\,\,\,\,\,\,\,\,\,\,\,\,\,\,\,\,\,\,\,\,\,\,\,\,\,\,\,\,\,\,\,\,\,\,\,\,\,\,\,\,\,\,\,\,\,\,\,\,=[-\frac{e^{-\lambda x}}{\lambda}]_{0}^{\infty}$

$\,\,\,\,\,\,\,\,\,\,\,\,\,\,\,\,\,\,\,\,\,\,\,\,\,\,\,\,\,\,\,\,\,\,\,\,\,\,\,\,\,\,\,\,\,\,\,\,\,\,\,\,\,=(0-(-\frac{1}{\lambda}))$

$\,\,\,\,\,\,\,\,\,\,\,\,\,\,\,\,\,\,\,\,\,\,\,\,\,\,\,\,\,\,\,\,\,\,\,\,\,\,\,\,\,\,\,\,\,\,\,\,\,\,\,\,\,=\frac{1}{\lambda}$

\vspace{10pt}

$\therefore \mathbb{E}X=\frac{1}{\lambda}$



\newpage
## Exercise 5



*Show that Var(X)=*$1/\lambda^2.$*(Hint: need to do *
$EX^2$ *first*)

\vspace{20pt}

$Var(X)=\mathbb{E}(X^2)-(\mathbb{E}(X))^2$
\vspace{10pt}

$\mathbb{E}(X^2)=\int_{-\infty}^{\infty}x^2f(x)\,\,dx=\int_{-\infty}^{0}x^2f(x)\,\,dx+\int_{0}^{\infty}x^2f(x)\,\,dx$

$\,\,\,\,\,\,\,\,\,\,\,\,\,\,\,\,\,\,\,\,\,\,\,\,\,\,\,\,\,\,\,\,\,\,\,\,\,\,\,\,\,\,\,\,\,\,\,\,\,\,\,\,\,\,\,\,\,\,\,\,\,\,\,=\int_{0}^{\infty}x^2\lambda e^{-\lambda x}\,\,dx$

$\,\,\,\,\,\,\,\,\,\,\,\,\,\,\,\,\,\,\,\,\,\,\,\,\,\,\,\,\,\,\,\,\,\,\,\,\,\,\,\,\,\,\,\,\,\,\,\,\,\,\,\,\,\,\,\,\,\,\,\,\,\,\,=\int_{0}^{\infty}\lambda x^2 e^{-\lambda x}\,\,dx$

$\,\,\,\,\,\,\,\,\,\,\,\,\,\,\,\,\,\,\,\,\,\,\,\,\,\,\,\,\,\,\,\,\,\,\,\,\,\,\,\,\,\,\,\,\,\,\,\,\,\,\,\,\,\,\,\,\,\,\,\,\,\,\,=[-x^2e^{-\lambda x}]_{0}^{\infty}-\int_{0}^{\infty}-2xe^{-\lambda x}\,\,dx$

$\,\,\,\,\,\,\,\,\,\,\,\,\,\,\,\,\,\,\,\,\,\,\,\,\,\,\,\,\,\,\,\,\,\,\,\,\,\,\,\,\,\,\,\,\,\,\,\,\,\,\,\,\,\,\,\,\,\,\,\,\,\,\,=(0-0)+\int_{0}^{\infty}2xe^{-\lambda x}\,\,dx$

$\,\,\,\,\,\,\,\,\,\,\,\,\,\,\,\,\,\,\,\,\,\,\,\,\,\,\,\,\,\,\,\,\,\,\,\,\,\,\,\,\,\,\,\,\,\,\,\,\,\,\,\,\,\,\,\,\,\,\,\,\,\,\,=2\int_{0}^{\infty}xe^{-\lambda x}\,\,dx$

$\,\,\,\,\,\,\,\,\,\,\,\,\,\,\,\,\,\,\,\,\,\,\,\,\,\,\,\,\,\,\,\,\,\,\,\,\,\,\,\,\,\,\,\,\,\,\,\,\,\,\,\,\,\,\,\,\,\,\,\,\,\,\,=2\{[-\frac{xe^{-\lambda x}}{\lambda}]_{0}^{\infty}-\int_{0}^{\infty}\frac{e^{-\lambda x}}{\lambda}\,\,dx\}$

$\,\,\,\,\,\,\,\,\,\,\,\,\,\,\,\,\,\,\,\,\,\,\,\,\,\,\,\,\,\,\,\,\,\,\,\,\,\,\,\,\,\,\,\,\,\,\,\,\,\,\,\,\,\,\,\,\,\,\,\,\,\,\,=2\{(0-0)-\int_{0}^{\infty}\frac{e^{-\lambda x}}{\lambda}\,\,dx\}$

$\,\,\,\,\,\,\,\,\,\,\,\,\,\,\,\,\,\,\,\,\,\,\,\,\,\,\,\,\,\,\,\,\,\,\,\,\,\,\,\,\,\,\,\,\,\,\,\,\,\,\,\,\,\,\,\,\,\,\,\,\,\,\,=2(-[\frac{e^{-\lambda x}}{\lambda^2}]_{0}^{\infty})$

$\,\,\,\,\,\,\,\,\,\,\,\,\,\,\,\,\,\,\,\,\,\,\,\,\,\,\,\,\,\,\,\,\,\,\,\,\,\,\,\,\,\,\,\,\,\,\,\,\,\,\,\,\,\,\,\,\,\,\,\,\,\,\,=2\times(0-(-\frac{1}{\lambda^2}))$

$\,\,\,\,\,\,\,\,\,\,\,\,\,\,\,\,\,\,\,\,\,\,\,\,\,\,\,\,\,\,\,\,\,\,\,\,\,\,\,\,\,\,\,\,\,\,\,\,\,\,\,\,\,\,\,\,\,\,\,\,\,\,\,=\frac{2}{\lambda^2}$
\vspace{5pt}

$Var(X)=\mathbb{E}(X^2)-(\mathbb{E}(X))^2=\frac{2}{\lambda^2}-(\frac{1}{\lambda})^2=\frac{1}{\lambda^2}$
\vspace{10pt}

$\therefore\,\,Var(X)=\frac{1}{\lambda^2}$



\newpage
## Exercise 6


*Prove the previous theorem*

\vspace{20pt}

$Claim,$ $\mathbb{P}(X>s+t \mid X>t)=\mathbb{P}(X > s)$
\vspace{15pt}

$\mathbb{P}(X>s+t \mid X>t)=\frac{\mathbb{P}(X>s+t,X>t)}{\mathbb{P}(X>t)}$

$\,\,\,\,\,\,\,\,\,\,\,\,\,\,\,\,\,\,\,\,\,\,\,\,\,\,\,\,\,\,\,\,\,\,\,\,\,\,\,\,\,\,\,\,\,\,\,\,\,\,\,\,\,\,\,\,=\frac{\mathbb{P}(X>s+t)}{\mathbb{P}(X>t)}$

$\,\,\,\,\,\,\,\,\,\,\,\,\,\,\,\,\,\,\,\,\,\,\,\,\,\,\,\,\,\,\,\,\,\,\,\,\,\,\,\,\,\,\,\,\,\,\,\,\,\,\,\,\,\,\,\,=\frac{1-\mathbb{P}(X\leq s+t)}{1-\mathbb{P}(X\leq t)}$

$\,\,\,\,\,\,\,\,\,\,\,\,\,\,\,\,\,\,\,\,\,\,\,\,\,\,\,\,\,\,\,\,\,\,\,\,\,\,\,\,\,\,\,\,\,\,\,\,\,\,\,\,\,\,\,\,=\frac{1-F(s+t)}{1-F(t)}$

$\,\,\,\,\,\,\,\,\,\,\,\,\,\,\,\,\,\,\,\,\,\,\,\,\,\,\,\,\,\,\,\,\,\,\,\,\,\,\,\,\,\,\,\,\,\,\,\,\,\,\,\,\,\,\,\,=\frac{1-(1-e^{-\lambda(s+t)})}{1-(1-e^{-\lambda(t)})}$

$\,\,\,\,\,\,\,\,\,\,\,\,\,\,\,\,\,\,\,\,\,\,\,\,\,\,\,\,\,\,\,\,\,\,\,\,\,\,\,\,\,\,\,\,\,\,\,\,\,\,\,\,\,\,\,\,=e^{-\lambda s}$

$\,\,\,\,\,\,\,\,\,\,\,\,\,\,\,\,\,\,\,\,\,\,\,\,\,\,\,\,\,\,\,\,\,\,\,\,\,\,\,\,\,\,\,\,\,\,\,\,\,\,\,\,\,\,\,\,=1-(1-e^{-\lambda s})=1-F(s)$

$\,\,\,\,\,\,\,\,\,\,\,\,\,\,\,\,\,\,\,\,\,\,\,\,\,\,\,\,\,\,\,\,\,\,\,\,\,\,\,\,\,\,\,\,\,\,\,\,\,\,\,\,\,\,\,\,=1-\mathbb{P}(X\leq s)$

$\,\,\,\,\,\,\,\,\,\,\,\,\,\,\,\,\,\,\,\,\,\,\,\,\,\,\,\,\,\,\,\,\,\,\,\,\,\,\,\,\,\,\,\,\,\,\,\,\,\,\,\,\,\,\,\,=\mathbb{P}(X>s)$
\vspace{10pt}

$\therefore\,\,\mathbb{P}(X>s+t \mid X>t)=\mathbb{P}(X > s)$


\newpage
## Exercise 7


*For X~poi*$(\lambda),$ *prove that* $\mathbb{E}X=\lambda.$

\vspace{20pt}

$\mathbb{E}X=\sum_{x=-\infty}^{\infty} xp(x)$ *(this is common for all discrete r.v.)*

$\,\,\,\,\,\,\,\,\,\,\,=\sum_{x=-\infty}^{\infty}\frac{x\times\lambda^xe^{-\lambda}}{x!}$

$\,\,\,\,\,\,\,\,\,\,\,=\lambda\sum_{x=-\infty}^{\infty}\frac{\lambda^{x-1}e^{-\lambda}}{(x-1)!}\,\,\,\,\,\,\,\,\,\,\,\,\,\,\,\,\,\,\,\,\,\,\,\,\,\,\,\,\,Let,\,\,\,k=x-1\,\,\,\,\,\,\,\, (x:1 -> \infty,\,\,\,\,\,\,k:0 -> \infty)$

$\,\,\,\,\,\,\,\,\,\,\,=\lambda\sum_{k=0}^{\infty}\frac{\lambda^{k}e^{-\lambda}}{k!}$

$\,\,\,\,\,\,\,\,\,\,\,=\lambda e^{-\lambda}\sum_{k=0}^{\infty}\frac{\lambda^k}{k!}\,\,\,\,\,\,\,\,\,\,\,\,\,\,\,\,\,\,\,\,\,\,\,\,\,\,\,\,\,\,\,\,\,\,\sum_{k=0}^{\infty}\frac{\lambda^k}{k!}=e^{\lambda}$

$\,\,\,\,\,\,\,\,\,\,\,=\lambda e^{-\lambda}\times e^{\lambda}$

$\,\,\,\,\,\,\,\,\,\,\,=\lambda$
\vspace{15pt}

$\therefore\,\,\mathbb{E}X=\lambda$


\newpage
## Exercise 8


*For X~U(20,40), evaluate*$\mathbb{E}[X \wedge 25]and\mathbb{E}[(25-X)^+].$

\vspace{20pt}

\[f(x)=
\begin{Bmatrix}
\frac{1}{20} \,\,(20\leq x\leq 40) \\ \\0 \,\,\,\,\,\,\,\,\,\,\,\,\, otherwise
\end{Bmatrix}
\]
\vspace{10pt}

1. $\mathbb{E}[X \wedge 25]=\int_{-\infty}^{\infty}(X\wedge25)\frac{1}{20}\,\,dx$

$\,\,\,\,\,\,\,\,\,\,\,\,\,\,\,\,\,\,\,\,\,\,\,\,\,\,\,\,\,\,\,\,\,\,\,\,\,\,\,\,\,=\int_{20}^{25}\frac{1}{20}x\,\,dx+\int_{25}^{40}25\times \frac{1}{20}\,\,dx$

$\,\,\,\,\,\,\,\,\,\,\,\,\,\,\,\,\,\,\,\,\,\,\,\,\,\,\,\,\,\,\,\,\,\,\,\,\,\,\,\,\,=[\frac{1}{40}x^2]_{20}^{25}+[\frac{5}{4}x]_{25}^{40}$

$\,\,\,\,\,\,\,\,\,\,\,\,\,\,\,\,\,\,\,\,\,\,\,\,\,\,\,\,\,\,\,\,\,\,\,\,\,\,\,\,\,=\frac{225}{40}+\frac{75}{4}$

$\,\,\,\,\,\,\,\,\,\,\,\,\,\,\,\,\,\,\,\,\,\,\,\,\,\,\,\,\,\,\,\,\,\,\,\,\,\,\,\,\,=\frac{195}{8}$
\vspace{15pt}

2. $\mathbb{E}[(25-X)^+]=\int_{-\infty}^{\infty}(25-X)^+\frac{1}{20}\,\,dx$

$\,\,\,\,\,\,\,\,\,\,\,\,\,\,\,\,\,\,\,\,\,\,\,\,\,\,\,\,\,\,\,\,\,\,\,\,\,\,\,\,\,\,\,\,\,\,\,\,\,\,=\int_{20}^{25}(25-X)\frac{1}{20}\,\,dx+\int_{25}^{40}0\times \frac{1}{20}\,\,dx$

$\,\,\,\,\,\,\,\,\,\,\,\,\,\,\,\,\,\,\,\,\,\,\,\,\,\,\,\,\,\,\,\,\,\,\,\,\,\,\,\,\,\,\,\,\,\,\,\,\,\,=[\frac{5}{4}x-\frac{1}{40}x^2]_{20}^{25}+0$

$\,\,\,\,\,\,\,\,\,\,\,\,\,\,\,\,\,\,\,\,\,\,\,\,\,\,\,\,\,\,\,\,\,\,\,\,\,\,\,\,\,\,\,\,\,\,\,\,\,\,=\frac{25}{4}-\frac{225}{40}$

$\,\,\,\,\,\,\,\,\,\,\,\,\,\,\,\,\,\,\,\,\,\,\,\,\,\,\,\,\,\,\,\,\,\,\,\,\,\,\,\,\,\,\,\,\,\,\,\,\,\,=\frac{5}{8}$
\vspace{15pt}

$\therefore\,\,\mathbb{E}[x \wedge 25] = \frac{195}{8},\,\,\,\mathbb{E}[(25-X)^+]=\frac{5}{8}$


\newpage
## Exercise 9


*For X~Poi(8)*

1. $\mathbb{P}(X=0)$

2. $\mathbb{P}(2\leq X\leq 4)$

3. $\mathbb{P}(X>2)$

\vspace{20pt}

$\ast\,\,\mathbb{P}(X)=\frac{8^{x}e^{-8}}{x!}\,\,\ast$
\vspace{10pt}

1. $\mathbb{P}(X=0)=\frac{8^{0}e^{-8}}{0!}$

$\,\,\,\,\,\,\,\,\,\,\,\,\,\,\,\,\,\,\,\,\,\,\,\,\,\,\,\,\,\,\,\,\,\,\,\,\,\,\,\,\,=e^{-8}$

2. $\mathbb{P}(2\leq X\leq 4)=\mathbb{P}(X\leq4)-\mathbb{P}(X<2)$

$\,\,\,\,\,\,\,\,\,\,\,\,\,\,\,\,\,\,\,\,\,\,\,\,\,\,\,\,\,\,\,\,\,\,\,\,\,\,\,\,\,\,\,\,\,\,\,\,\,\,\,\,=\mathbb{P}(X=2)+\mathbb{P}(X=3)+\mathbb{P}(X=4)$

$\,\,\,\,\,\,\,\,\,\,\,\,\,\,\,\,\,\,\,\,\,\,\,\,\,\,\,\,\,\,\,\,\,\,\,\,\,\,\,\,\,\,\,\,\,\,\,\,\,\,\,\,=\frac{8^{2}e^{-8}}{2!}+\frac{8^{3}e^{-8}}{3!}+\frac{8^{4}e^{-8}}{4!}$

$\,\,\,\,\,\,\,\,\,\,\,\,\,\,\,\,\,\,\,\,\,\,\,\,\,\,\,\,\,\,\,\,\,\,\,\,\,\,\,\,\,\,\,\,\,\,\,\,\,\,\,\,=288e^{-8}$

3. $\mathbb{P}(X>2)=1-(\mathbb{P}(X=0)+\mathbb{P}(X=1)+\mathbb{P}(X=2))$

$\,\,\,\,\,\,\,\,\,\,\,\,\,\,\,\,\,\,\,\,\,\,\,\,\,\,\,\,\,\,\,\,\,\,\,\,\,\,\,\,\,=1-(\frac{8^{0}e^{-8}}{0!}+\frac{8^{1}e^{-8}}{1!}+\frac{8^{2}e^{-8}}{2!})$

$\,\,\,\,\,\,\,\,\,\,\,\,\,\,\,\,\,\,\,\,\,\,\,\,\,\,\,\,\,\,\,\,\,\,\,\,\,\,\,\,\,=1-41e^{-8}$
\vspace{15pt}

\[\therefore Answer:
\begin{Bmatrix}
\mathbb{P}(X=0)= e^{-8}\\ \\
\mathbb{P}(2\leq X\leq 4)= 288e^{-8}\\ \\
\mathbb{P}(X>2)=1-41e^{-8}
\end{Bmatrix}
\]


\newpage
## Exercise 10


*For X~exp(7), evaluate*$\mathbb{E}[max(X,7)].$

\vspace{20pt}

$\ast \,\, f(x)=7e^{-7x}$

\vspace{10pt}

$\mathbb{E}[max(X,7)]=\int_{-\infty}^{\infty}xf(x)\,\,dx$

$\,\,\,\,\,\,\,\,\,\,\,\,\,\,\,\,\,\,\,\,\,\,\,\,\,\,\,\,\,\,\,\,\,\,\,\,=\int_{-\infty}^{7}7\times 7e^{-7x}\,\,dx+\int_{7}^{\infty}x\times 7e^{-7x}\,\,dx$

$\,\,\,\,\,\,\,\,\,\,\,\,\,\,\,\,\,\,\,\,\,\,\,\,\,\,\,\,\,\,\,\,\,\,\,\,=\int_{0}^{7}49e^{-7x}\,\,dx+\int_{7}^{\infty}7xe^{-7x}\,\,dx$

$\,\,\,\,\,\,\,\,\,\,\,\,\,\,\,\,\,\,\,\,\,\,\,\,\,\,\,\,\,\,\,\,\,\,\,\,=[-7e^{-7x}]_{0}^{7}+[-xe^{-7x}]_{7}^{\infty}-\int_{7}^{\infty}-e^{-7x}\,\,dx$

$\,\,\,\,\,\,\,\,\,\,\,\,\,\,\,\,\,\,\,\,\,\,\,\,\,\,\,\,\,\,\,\,\,\,\,\,=(-7e^{-49}-(-7))+(0-(-7e^{-49}))+\int_{7}^{\infty}e^{-7x}\,\,dx$

$\,\,\,\,\,\,\,\,\,\,\,\,\,\,\,\,\,\,\,\,\,\,\,\,\,\,\,\,\,\,\,\,\,\,\,\,=7+[-\frac{e^{-7x}}{7}]_{7}^{\infty}$

$\,\,\,\,\,\,\,\,\,\,\,\,\,\,\,\,\,\,\,\,\,\,\,\,\,\,\,\,\,\,\,\,\,\,\,\,=7+(0-(-\frac{e^{-49}}{7}))$

$\,\,\,\,\,\,\,\,\,\,\,\,\,\,\,\,\,\,\,\,\,\,\,\,\,\,\,\,\,\,\,\,\,\,\,\,=7+\frac{e^{-49}}{7}$

\vspace{15pt}

$\therefore\,\,\,\mathbb{E}[max(X,7)]=7+\frac{e^{-49}}{7}$





\newpage
## Exercise 11


*For X~exp(8),find*$x^*$ *such that* $F(x^*)=0.6.$


\vspace{20pt}

\[f(x)=
\begin{Bmatrix}
8e^{-8x} \,\,\,\,\,\,(x\leq 0) \\ \\
0 \,\,\,\,\,\,\,\,\,\,\,\,\, otherwise
\end{Bmatrix}
\]
\vspace{10pt}

\[F(x)=
\begin{Bmatrix}
1-e^{-8x} \,\,\,\,\,\,(x\leq 0) \\ \\
0 \,\,\,\,\,\,\,\,\,\,\,\,\, otherwise
\end{Bmatrix}
\]

\vspace{15pt}

$F(x^*)=1-e^{-8x}=0.6$

$\,\,\,\,\,\,\,\,\,\,\,\,\,\,\,\,\,\,\,\,\,\,\,e^{-8x^*}=0.4$

$\,\,\,\,\,\,\,\,\,\,\,\,\,\,\,\,\,\,\,\,\,\,\,\frac{1}{e^{8x^*}}=\frac{2}{5}$

$\,\,\,\,\,\,\,\,\,\,\,\,\,\,\,\,\,\,\,\,\,\,\,e^{8x^*}=\frac{5}{2}$

*Taking the ln(x) on both side*

$\,\,\,\,\,\,\,\,\,\,\,\,\,\,\,\,\,\,\,\,\,\,\,8x^*=ln(\frac{5}{2})=ln5-ln2$
\vspace{10pt}

$\,\,\,\,\,\,\,\,\,\,\,\,\,\,\,\,\,\,\,\,\,\therefore x^*=\frac{ln5-ln2}{8}$








\newpage
## Exercise 12


*For X~U(10,20),find*$x^*$ *such that* $F(x^*)=0.7.$

\vspace{20pt}

\[F(x)=
\begin{Bmatrix}
0 \,\,\,\,\,\,\,\,\,\,\,\,\,\,\,\,\,(10\leq x) \\ \\ \frac{x-10}{10} \,\,\,\,\,\,\,(10\leq x \leq 20) \\
\\1 \,\,\,\,\,\,\,\,\,\,\,\,\,(x>20)
\end{Bmatrix}
\]

$\ast F(x^*)=0.7$

*For getting the value 0.7,*$x^*$*should be between 10 and 20, Because the other ranges have value only 0 or 1*

\vspace{10pt}

$F(x^*)=\frac{x^*-10}{10}=0.7$

$\,\,\,\,\,\,\,\,x^*-10=7$

$\,\,\,\,\,\,\,\therefore \,\,x^*=17$







