---
title: "A1_3,4"
author: "Son Min Sang"
date: "`r Sys.Date()`"  
output:   
  pdf_document:  
    latex_engine: xelatex
    highlight: haddock  
    keep_tex: true  
    includes:
    #in_header: rmd-pdf-support/latex-topmatter.tex
    # pandoc_args: [
    #  "-V", "classoption=twocolumn"
    # ]
    toc: true   
    toc_depth: 2  
    # number_sections: true  
monofont: Consolas
smaller: yes
classoption: a4paper
---

```{r setup, include=FALSE}
knitr::opts_chunk$set(echo = FALSE)
knitr::opts_chunk$set(background = '718CBA')


```

## Exercise 3

Derive $\int{f'(x)g(x) dx} = f(x)g(x) - \int{f(x)g'(x) dx}.$(Hint: Use Theorem 2 above.)

### Solution

$(f(x)·g(x))' =f'(x)g(x)+f(x)g'(x)$

\vspace{10pt}

\bf{ antiderivative}

$f(x)·g(x) =\int f'(x)g(x)dx+\int f(x)g'(x)dx$

$\int f'(x)g(x)dx=f(x)g(x)-\int f(x)g'(x)dx$

\vspace{20pt}

## Exercise 4 

Find $\int{xe^xdx}$,and evaluate $\int_{0}^{1}{xe^x}dx$.(Hint: Use Exercise 3 above.)

### Solution

\bf {Exercise 3}

$\int f'(x)g(x)dx=f(x)·g(x)-\int f(x)g'(x)dx$

\vspace{10pt}


$\int xe^xdx=e^xx-\int (e^x·1)dx$

\qquad \qquad $=e^xx-e^x+Cdx$

\vspace{10pt}

$\int_{0}^{1} xe^xdx=[e^xx-e^x+C]_0^1$

\qquad \qquad $=(e^1·1-e^1+C)-(e^0·0-e^0+C)$

\qquad \qquad $=(0+C)-(0-1+C)$

\qquad \qquad $=1$
