---
title: "Lecture A1 Solution"  
author: "Reinforcement Learning Study"  
date: "`r Sys.Date()`"  
output:   
  pdf_document:  
    latex_engine: xelatex
    highlight: haddock  
    keep_tex: true  
    includes:
      in_header: rmd-pdf-support/latex-topmatter.tex
    # pandoc_args: [
    #  "-V", "classoption=twocolumn"
    # ]
    toc: True   
    toc_depth: 2  
    # number_sections: true  
monofont: Consolas
smaller: yes
classoption: a4paper
header-includes: 
  - \usepackage{tikz}
  - \usepackage{pgfplots}
---

```{r setup, include=FALSE}
knitr::opts_chunk$set(echo = TRUE)


```

\newpage 

## Exercise 1


Problem : Suppose $f(x)=xe^x$, find $f'(x)$.


  $f(x)=xe^x$

  $f'(x)=(x)'e^x+x(e^x)'$
  
  
  $\therefore,\,\, f'(x)=e^x+xe^x$



## Exercise 2


Problem : Suppose $f(x)=e^{2x}$, find $f'(x)$.


def $f(x)=h(g(x))$

  $f(x)=e^{2x} => h(x)=e^x,\,\,g(x)=2x$

$\therefore, \,\,f'(x)=e^{2x}\times 2 = 2e^{2x}$


## Exercise 3

Derive $\int{f'(x)g(x) dx} = f(x)g(x) - \int{f(x)g'(x) dx}.$(Hint: Use Theorem 2 above.)

### Solution

$(f(x)·g(x))' =f'(x)g(x)+f(x)g'(x)$

\vspace{10pt}

\bf{ antiderivative}

$f(x)·g(x) =\int f'(x)g(x)dx+\int f(x)g'(x)dx$

$\int f'(x)g(x)dx=f(x)g(x)-\int f(x)g'(x)dx$

\vspace{20pt}

## Exercise 4 

Find $\int{xe^xdx}$,and evaluate $\int_{0}^{1}{xe^x}dx$.(Hint: Use Exercise 3 above.)

### Solution

\bf {Exercise 3}

$\int f'(x)g(x)dx=f(x)·g(x)-\int f(x)g'(x)dx$

\vspace{10pt}


$\int xe^xdx=e^xx-\int (e^x·1)dx$

\qquad \qquad $=e^xx-e^x+Cdx$

\vspace{10pt}

$\int_{0}^{1} xe^xdx=[e^xx-e^x+C]_0^1$

\qquad \qquad $=(e^1·1-e^1+C)-(e^0·0-e^0+C)$

\qquad \qquad $=(0+C)-(0-1+C)$

\qquad \qquad $=1$


## Exercise 5

Solve the followings
$$
\left(\begin{array}{cc} 
.6 & .4\\
\end{array}\right)
\left(\begin{array}{cc} 
.7 & .3\\ 
.5 & .5
\end{array}\right) =
$$ 
$$
\left(\begin{array}{cc} 
0.6*0.7+0.4*0.5 & 0.6*0.4+0.4*0.5\\
\end{array}\right) = 
\left(\begin{array}{cc} 
0.62 & 0.38.\\
\end{array}\right)
$$



## Exercise 6

What is $P^2$?

$$
P=
\left(\begin{array}{cc} 
.7 & .3\\ 
.5 & .5
\end{array}\right)
$$ 
$$
P=
\left(\begin{array}{cc} 
0.7 & 0.3\\ 
0.5 & 0.5
\end{array}\right) 
\left(\begin{array}{cc} 
0.7 & 0.3\\ 
0.5 & 0.5
\end{array}\right) = 
\left(\begin{array}{cc} 
0.74 & 0.36\\ 
0.6 & 0.4
\end{array}\right)
$$ 


## Exercise 7

#### Solve the followings.  


\vspace{15pt}
$$\left(
\begin{array}{cc}
\pi_{1}&\pi_{2}
\end{array}\right)
\left(\begin{array}{cc}
.7&.3 \\
.5&.5
\end{array}\right)
\left(
\begin{array}{cc}
\pi_{1}&\pi_{2}
\end{array}
\right)$$

\begin{center}
$\pi_{1}+\pi_{2}=1$
\end{center}

\vspace{15pt}

(1)
\begin{eqnarray*}
0.7\pi_{1}+0.5\pi_{2}&=&\pi_{1}\\
 \\
0.5\pi_{2}&=&0.3\pi_{1} \\
 \\
\pi_{2}&=&0.6\pi_{1}
\end{eqnarray*}

(2)
\begin{eqnarray*}
\pi_{1}+\pi_{2}=1
\end{eqnarray*}

**From(1) & (2),**
  
  
$\pi_{1}+0.6\pi_{1}=1$  


Thus,  $\pi_{1}=\frac{5}{8}$, $\pi_{2}=\frac{3}{8}$.

\newpage

## Exercise 8

#### Solve the following system of equations.

\begin{eqnarray*}
(1)　　x&=&y \\
 \\
(2)　　y&=&0.5z \\
 \\
(3)　　z&=&0.6-0.4x \\
 \\
(4)　　x+y+z&=&1
\end{eqnarray*}

**From (1) & (2) & (4),**
  
\begin{eqnarray*}
y+y+z&=&1 \\
 \\
2y+z&=&1 \\
 \\
z+z&=&1 \\
 \\
z&=&\frac{1}{2}
\end{eqnarray*}

Thus, $x=\frac{1}{4}, y=\frac{1}{4}, z=\frac{1}{2}$


## Exercise 9
**Solve the following system of equations.**
$$
\begin{pmatrix} \pi_0 & \pi_1 & \pi_2 \end{pmatrix}
\begin{pmatrix} -2 & 2 \\ 3 & -5 & 2 \\ & 3 &-3 \end{pmatrix} =
\begin{pmatrix} 0 & 0 & 0 \end{pmatrix}
$$
$$ \pi_0 + \pi_1 + \pi_2 = 1 $$

\vspace{50pt}
$$
\begin{pmatrix} \pi_0 & \pi_1 & \pi_2 \end{pmatrix}
\begin{pmatrix} -2 & 2 \\ 3 & -5 & 2 \\ & 3 &-3 \end{pmatrix} =
\begin{pmatrix} -2\pi_0+3\pi_1 & 2\pi_0-5\pi_1+3\pi_2 & 2\pi_1-3\pi_2 \end{pmatrix}
$$

\begin{align}
  -2\pi_0+3\pi_1= 0 \\
  2\pi_0-5\pi_1+3\pi_2 = 0 \\
  2\pi_1-3\pi_2 = 0 \\
  \pi_0 + \pi_1 + \pi_2 = 1
\end{align}

(1) equals $\pi_0=\frac{3}{2}\pi_1$.
(3) equals $\pi_2=\frac{3}{2}\pi_1$.
Using above two equations, (4) equals $\frac{3}{2}\pi_1+\pi_1+\frac{2}{3}\pi_1=1$.
Thus, $\pi_1=\frac{6}{19}$.

Using (1), $\pi_0=\frac{9}{19}$.
Using (3), $\pi_2=\frac{4}{19}$.

(2) equals $\frac{18}{19}-\frac{30}{19}+\frac{12}{19}=0$.

$\therefore \pi_0=\frac{9}{19}$, $\pi_1=\frac{6}{19}$, $\pi_2=\frac{4}{19}$.


## Exercise 10
**Solve the following system of equations.**
$$
\begin{pmatrix} \pi_1 & \pi_2 & \pi_3 & \pi_4 \end{pmatrix}  
\begin{pmatrix} .7 & .3 \\ .5 & .5 \\ & & .6 & .4 \\ & & .3 & .7 \end{pmatrix} = 
\begin{pmatrix} \pi_1 & \pi_2 & \pi_3 & \pi_4 \end{pmatrix} 
$$

$$
\pi_1 + \pi_2 + \pi_3 + \pi_4 = 1 \\

\pi_1 + \pi_2 = \alpha
$$

\begin{align}
  0.7\pi_1 + 0.5\pi_2 = \pi_1 \\
  0.3\pi_1 + 0.5\pi_2 = \pi_2 \\
  0.6\pi_3 + 0.3\pi_4 = \pi_3 \\
  0.4\pi_3 + 0.7\pi_4 = \pi_4
\end{align}

(5) equals $5\pi_2 = 3\pi_1$.
(6) equals $3\pi_1 = 5\pi_2$.
(7) equals $4\pi_3 = 3\pi_4$.
(8) equals $4\pi_3 = 3\pi_4$.


By using (5) and (6), $\pi_2=\frac{3}{5}\pi_1$.
By using (7) and (8), $\pi_4=\frac{4}{3}\pi_3$.


\begin{align}
  \pi_1 + \pi_2 + \pi_3 + \pi_4 = \pi_1 + \frac{3}{5}\pi_1 + \pi_3 + \frac{4}{3}\pi_3 = \frac{3}{5}\pi_1 + \frac{7}{3}\pi_3 =  1
\end{align}

(9) equals $\pi_3=\frac{3}{7}-\frac{24}{35}\pi_1$.

Thus, $\pi_4 = \frac{4}{7}-\frac{32}{35}\pi_1$.

$$ 
\therefore \pi_1 = \frac{5}{8}\alpha,
\pi_2 = \frac{3}{8}\alpha, 
\pi_3 = \frac{3}{7}-\frac{3}{7}\alpha, 
\pi_4 = \frac{4}{7}-\frac{4}{7}\alpha 
$$


## Exercise 11

Solve following and express $\pi_i$ for $i=0,1,2,...$
\begin{eqnarray}
\pi_0 + \pi_1 + \pi_2 +... &=& 1 \nonumber\\
0.02 \pi_0 + 0.02 \pi_1 + 0.02 \pi_2 + ... &=& \pi_0 \nonumber\\
0.98 \pi_0 &=& \pi_1 \nonumber\\
0.98 \pi_1 &=& \pi_2 \nonumber\\
0.98 \pi_2 &=& \pi_3 \nonumber\\
...&=&... \nonumber
\end{eqnarray}

### Solution:

\begin{eqnarray}
\pi_0 + \pi_1 + \pi_2 +... &=& 1 \\
0.02 \pi_0 + 0.02 \pi_1 + 0.02 \pi_2 + ... &=& \pi_0 \\
0.98 \pi_0 &=& \pi_1 \\
0.98 \pi_1 &=& \pi_2 \\
0.98 \pi_2 &=& \pi_3 \\
...&=&... \nonumber
\end{eqnarray}


From (3)-(5), 

\begin{eqnarray}
\pi_1 &=& (0.98)\pi_0 \nonumber\\
\pi_2 &=& (0.98)\pi_1 = (0.98)^2 \pi_0 \nonumber\\
\pi_3 &=& (0.98)\pi_2 = (0.98)^3 \pi_0 \nonumber\\
\pi_i &=& (0.98)^i \pi_0\nonumber
\end{eqnarray}

Thus (1), becomes 

\begin{eqnarray*}
\pi_0 + \pi_1 + \pi_2 +... &=& \pi_0(1+0.98+0.98^2 + ...) \nonumber\\
\pi_0 (\frac{1}{1-0.98})) &=& 1 \nonumber\\
\pi_0 &=& 0.02\nonumber\\
\therefore \pi_i &=& (0.02)(0.98)^i \nonumber
\end{eqnarray*}

\newpage 

## Excercise 12 (Infinite geometric series)

Simplify the following. When $|r|<1$, $S=a+ar+ar^2+ar^3+...$

### Solution :

\setcounter{equation}{0}

\begin{eqnarray}
S  &=& a+ar^2+ar^3+...      \\
rS &=&   ar^2+ar^3+ar^4+...  \\
\nonumber
\end{eqnarray}

Subtract (1) and (2)

$(1-r)S = a$

$\therefore   S = \frac{a}{1-r}$

## Exercise 13 (Finite geometric series)

### Simplify the following. When $r\neq 1, S = a+ar+ar^2+ar^3+ ... +ar^{n-1}$

### Solution:

$S = a+ar+ar^2+ ... +ar^{n-1}$

$rS = ar+ar^2+ar^3+ ... +ar^{n}$

$S-rs = a-ar^n$

$S=\frac{a(1-r^n)}{(1-r)}$

## Exercise 14 (Power series)

### Simplify the following. When $|r|\neq 1, S = r+2r^2+3r^3+4r^4+ ...$

### Solution:


$S = r+2r^2+3r^3+4r^4+ ...$

$rS = r^2+2r^3+3r^4+...$

$(1-r)S=r+r^2+r^3+...$

$(1-r)S=\frac{r}{1-r}$

$S=\frac{r}{(1-r)^2}$


## Exercise 15

### During the first hour $(0\leq t \geq 1), \lambda(t)$ increases linearly from 0 to 60. After the first hour, $\lambda(t)$ is constant at 60. Draw plot for $\lambda(t)$ and express the function in math form.

### Solution:

$\lambda(t) = \begin{cases}60t & t\le 60 \\60 &t>60 \end{cases}$

![graph](C://Users/user/Desktop/A1/A1_solution_latex/graph.png)

```{r, results='hide'}
"A1_Solution"
```
